Update SequenceNumbers.dfy

SequenceNumbers.dfy
@@ -14,61 +14,190 @@ method Max(a: int, b:int) returns (c: int)
 
 type byte = x | 0 <= x < 256
 
-predicate BitVector_Less(bi1: byte, bi2:byte)
+predicate LessThan(bi1: byte, bi2:byte)
 {
-    (bi1 < bi2 && (bi2 - bi1) < 128) || (bi1 > bi2 && (bi1 - bi2) > 128)
+    (bi1 < bi2 && (bi2 - bi1) < 128) 
+    || 
+    (bi1 > bi2 && (bi1 - bi2) > 128)
+}
+
+predicate Simple_less(bi1: int, bi2:int)
+{
+    bi1 < bi2
+}
+
+predicate LessThanOrig(bi1: byte, bi2:byte)
+{
+    !(((bi1 > 128) && (bi1 > bi2 && bi2 > bi1 - 128)) 
+    ||
+    ((bi1 <= 128) && (bi1 > bi2 || bi2 > bi1 + 128)))
+}
+
+predicate LessThanFixed(bi1: byte, bi2:byte)
+{
+    !(((bi1 > 128) && (bi1 >= bi2 && bi2 >= bi1 - 128)) 
+    ||
+    ((bi1 <= 128) && (bi1 >= bi2 || bi2 >= bi1 + 128)))
+}
+
+lemma Shift(bi1: byte, bi2:byte, bi3: byte)
+ensures LessThan(bi1, bi2) == LessThan((bi1 + bi3) % 256, (bi2 + bi3) % 256)
+{
+
+}
+
+lemma Shiftn(i1: int, i2:int, i3: int)
+    ensures Simple_less(i1, i2)  == (Simple_less(i1 - i3 ,i2 - i3))
+{
+
+}
+
+lemma Compare0(bi1: byte, bi2:byte)
+    requires bi1 > 128 && bi2 > bi1 - 128
+    ensures Simple_less(bi1, bi2) ==> LessThanFixed(bi1, bi2)
+{
+
+}
+
+lemma Compare1(bi1: byte, bi2:byte)
+    ensures LessThan(bi1, bi2) ==> LessThanFixed(bi1, bi2)
+{
+
+}
+
+lemma Compare2(bi1: byte, bi2:byte)
+    requires bi2 - bi1 !=  128 && bi2 - bi1 !=  -128 && bi1 != bi2
+    ensures LessThanFixed(bi1, bi2) ==> LessThan(bi1, bi2)
+{
+
+}
+
+lemma Compare2a(bi1: byte, bi2:byte)
+    ensures LessThanFixed(bi1, bi2) ==> (LessThan(bi1, bi2))
+{
+
+}
+
+lemma Compare3(bi1: byte, bi2:byte)
+    ensures LessThanFixed(bi1, bi2) <==> (LessThan(bi1, bi2))
+{
+
+}
+
+lemma Shift2(bi1: byte, bi2:byte, bi3: byte)
+    requires bi2 - bi1 !=  128 && bi1 - bi2 !=  128 
+ensures LessThanFixed(bi1, bi2) == LessThanFixed((bi1 + bi3) % 256, (bi2 + bi3) % 256)
+{
+
+}
+
+lemma Compare4(i1: nat, i2:nat)
+    requires -128 < i1 - i2 < 128
+	ensures i1 < i2 ==> LessThan(i1 % 256, i2 % 256)
+	ensures i2 < i1 ==> LessThan(i2 % 256, i1 % 256)
+{
+
+}
+
+lemma Compare5(i1: nat, i2:nat)
+    requires -128 < i1 - i2 < 128
+	ensures i1 < i2 ==> LessThanFixed(i1 % 256, i2 % 256)
+	ensures i2 < i1 ==> LessThanFixed(i2 % 256, i1 % 256)
+{
+
+}
+
+lemma transn(i1: int, i2:int, i3: int)
+ensures (i1 < i2) && (i2 < i3) ==> (i1 < i3)
+{
+
+}
+
+lemma trans(bi1: byte, bi2:byte, bi3: byte)
+requires -64 < bi1 - bi2 < 128 && -64 < bi2 - bi3 < 128
+ensures LessThan(bi1, bi2) && LessThan(bi2, bi3) ==> LessThan(bi1, bi3)
+{
+
+}
+
+datatype Threeway = equivalent | less | greater | unordered
+
+function ThreeWay(i1: byte, i2:byte) :Threeway
+{
+    if (i1 == i2) then  equivalent
+    else if (LessThan(i1, i2)) then less
+    else if (LessThan(i2, i1)) then greater
+    else unordered
+}
+
+function ThreeWay2(i1: byte, i2:byte) :Threeway
+{
+    if (i1 == i2) then  equivalent    
+    else if (LessThan(i1, i2)) then less
+    else if (LessThan(i2, i1)) then greater
+    else unordered
+}
+
+lemma compareTwoLess(i1: byte, i2:byte)
+    ensures ThreeWay(i1, i2) == less <== ThreeWay2(i1, i2) == less
+{
+
+}
+
+lemma compareTwoGreater(i1: byte, i2:byte)
+    ensures ThreeWay(i1, i2) == greater <== ThreeWay2(i1, i2) == greater
+{
+
+}
+
+lemma compareTwoEquiv(i1: byte, i2:byte)
+    ensures ThreeWay(i1, i2) == equivalent ==> ThreeWay2(i1, i2) == equivalent
+{
+
 }
 
 datatype Option<+T> = Nil | Some(Data: T)
 
 method MinMax(i1: byte, i2:byte) returns (Min: Option<byte>, Max: Option<byte>)
-	ensures BitVector_Less(i1, i2) ==> Max == Some((i2 % 256) as byte) && Min == Some((i1 % 256) as byte) 
-	ensures BitVector_Less(i2, i1) ==> Max == Some((i1 % 256) as byte) && Min == Some((i2 % 256) as byte)
+	ensures LessThan(i1, i2) ==> Max == Some((i2 % 256) as byte) && Min == Some((i1 % 256) as byte) 
+	ensures LessThan(i2, i1) ==> Max == Some((i1 % 256) as byte) && Min == Some((i2 % 256) as byte)
     ensures i2 == i1 ==> Max == Some((i1 % 256) as byte) && Min == Some((i2 % 256) as byte)
-    ensures (!BitVector_Less(i1, i2) && !BitVector_Less(i2, i1) && !(i2 == i1)) ==> Max == Nil && Min == Nil
+    ensures (!LessThan(i1, i2) && !LessThan(i2, i1) && !(i2 == i1)) ==> Max == Nil && Min == Nil
 {
-	if (BitVector_Less(i1, i2)) 
+    match ThreeWay(i1, i2)
     {
-        Max, Min := Some(i2), Some(i1);
-	} 
-    else if (BitVector_Less(i2, i1))
-    {
-        Max, Min := Some(i1), Some(i2);
-	}
-    else if (i2 == i1)
-    {
-        Max, Min := Some(i1), Some(i2);
-    }
-    else
-    {
-        Max, Min:= Nil, Nil;
+        case less => Max, Min := Some(i2), Some(i1);
+        case greater => Max, Min :=  Some(i1), Some(i2);
+        case equivalent => Max, Min := Some(i1), Some(i2);     
+        case unordered => Max, Min := Nil, Nil;
     }
 }
 
 method MinMax2(i1: byte, i2:byte) returns (Min: byte, Max: byte)
-	ensures BitVector_Less(i1, i2) ==> Max == (i2 % 256) as byte && Min == (i1 % 256) as byte 
-	ensures BitVector_Less(i2, i1) ==> Max == (i1 % 256) as byte && Min == (i2 % 256) as byte
-    ensures (!BitVector_Less(i1, i2) && !BitVector_Less(i2, i1)) ==> Max == (i1 % 256) as byte && Min == (i2 % 256) as byte
+	ensures LessThan(i1, i2) ==> Max == (i2 % 256) as byte && Min == (i1 % 256) as byte 
+	ensures LessThan(i2, i1) ==> Max == (i1 % 256) as byte && Min == (i2 % 256) as byte
+    ensures (!LessThan(i1, i2) && !LessThan(i2, i1)) ==> Max == (i1 % 256) as byte && Min == (i2 % 256) as byte
 {
-	if (BitVector_Less(i1, i2)) 
-    {
-        Max, Min := i2, i1;
-	} 
-    else 
-    {
-        Max, Min := i1, i2;
-	}
+   match ThreeWay(i1, i2)
+   {
+        case less => Max, Min := i2, i1;
+        case greater => Max, Min := i1, i2;
+        case equivalent => Max, Min := i1, i2;        
+        case unordered => Max, Min := i1, i2;
+    }
 }
 
 method SequenceNumberMinMax(i1: nat, i2:nat) returns (Min: byte, Max: byte)
-    requires -128 < i1 - i2 < 129
+    requires -128 < i1 - i2 < 128
 	ensures i1 < i2  ==> Max == (i2 % 256) as byte && Min == (i1 % 256) as byte 
 	ensures i2 <= i1 ==> Max == (i1 % 256) as byte && Min == (i2 % 256) as byte 
 {
     var bi1 := (i1 % 256) as byte;
     var bi2 := (i2 % 256) as byte;
-    var MinOpt2, MaxOpt2 := MinMax2(bi1, bi2);    
-    Max, Min := MaxOpt2, MinOpt2;
+    var MinOpt2, MaxOpt2 := MinMax(bi1, bi2);    
+    assert(MinOpt2 != Nil && MaxOpt2 != Nil);
+    Max, Min := MaxOpt2.Data, MinOpt2.Data;
+
 }
 
 method TestMax()
@@ -91,13 +220,18 @@ method TestMax()
     assert(44 == MaxTest4);   
     assert(0 == Mintest4);   
 
-    var ll := BitVector_Less(128, 0);
-    var ll1 := BitVector_Less(0, 128);
-    assert(!ll1); // unordered     
-    assert(!ll);   
+    assert(LessThan(128, 0) == LessThan(0, 128));// unordered     
+    assert(LessThan(128, 1) == LessThan(0, 129));       
+    var ll := LessThan(128, 0) ;
+    assert(!ll); // unordered     
 
-    var ll2 := BitVector_Less(255, 0);
-    var ll3 := BitVector_Less(0, 255);
+    assert(LessThanFixed(128, 0) == LessThanFixed(0, 128));// ordered     
+    assert(LessThanFixed(128, 1) == LessThanFixed(0, 129));   
+    var wll := LessThanFixed(128, 0);
+    assert(!wll);       
+
+    var ll2 := LessThan(255, 0);
+    var ll3 := LessThan(0, 255);
     assert(ll2); // ordered     
     assert(!ll3);   
 
@@ -108,5 +242,5 @@ method TestMax()
     assert(Mini == Nil); // unordered     
     assert(Maxi == Nil); // unordered       
 
-    assert(!BitVector_Less(1, 1));
+    assert(!LessThan(1, 1));
 }
